DCE.v
@@ -194,21 +194,132 @@ Proof.
   intros EQ. eapply LenNEq. rewrite <- EQ. reflexivity.
 Qed.
 
+Lemma override P : P -> True.
+  eauto.
+Qed.
+
+Tactic Notation "override" hyp(H) := apply override in H.
+
+Lemma DVE_callChain RL ZL F als t alt l' k ZsEnd aEnd n
+      (IH : forall k Zs,
+          get F k Zs ->
+       forall (ZL : 〔params〕) (RL : 〔bool〕) (lv : ann bool) (n : nat),
+       unreachable_code SoundAndComplete ZL RL (snd Zs) lv ->
+       trueIsCalled (snd Zs) (LabI n) ->
+       getAnn lv ->
+       isCalled (compile (pair ⊜ RL ZL) (snd Zs) lv)
+                (LabI (countTrue (fst ⊝ take n (pair ⊜ RL ZL)))))
+  (UC:unreachable_code SoundAndComplete (fst ⊝ F ++ ZL) (getAnn ⊝ als ++ RL) t alt)
+  (LEN: ❬F❭ = ❬als❭)
+  (UCF:forall (n : nat) (Zs : params * stmt) (a : ann bool),
+       get F n Zs ->
+       get als n a ->
+       unreachable_code SoundAndComplete (fst ⊝ F ++ ZL)
+         (getAnn ⊝ als ++ RL) (snd Zs) a)
+  (Ann: getAnn alt)
+  (IC: trueIsCalled t (LabI l'))
+  (CC: callChain trueIsCalled F (LabI l') (LabI k))
+  (GetF: get F k ZsEnd)
+  (ICEnd: trueIsCalled (snd ZsEnd) (LabI (❬F❭ + n)))
+  (GetAls: get als k aEnd)
+: callChain isCalled
+            (compileF compile (pair ⊜ (getAnn ⊝ als ++ RL) (fst ⊝ F ++ ZL)) F als)
+            (LabI (countTrue (fst ⊝ take l' (pair ⊜ (getAnn ⊝ als ++ RL)
+                                                  (fst ⊝ F ++ ZL)))))
+            (LabI (countTrue (getAnn ⊝ als) +
+                   countTrue (fst ⊝ take n (pair ⊜ RL ZL)))).
+Proof.
+  general induction CC.
+  - exploit unreachable_code_trueIsCalled as IMPL; try eapply IC; eauto.
+    simpl in *; dcr; inv_get. rewrite H1 in Ann.
+    exploit compileF_get; eauto.
+    eapply Is_true_eq_true; eauto.
+    econstructor 2; [ | | econstructor 1 ].
+    rewrite zip_app at 2; eauto with len.
+    rewrite take_app_lt; eauto 20 with len.
+    rewrite map_take. rewrite <- getAnn_eq; eauto.
+    rewrite <- map_take. eauto. simpl.
+    eapply IH in ICEnd; eauto.
+    rewrite zip_app in ICEnd; eauto with len.
+    rewrite take_app_ge in ICEnd; eauto 20 with len.
+    rewrite zip_length2 in ICEnd; eauto with len.
+    rewrite map_length in ICEnd.
+    orewrite (❬F❭ + n - ❬als❭ = n) in ICEnd. simpl.
+    rewrite map_app in ICEnd. rewrite countTrue_app in ICEnd.
+    rewrite <- getAnn_eq in ICEnd; eauto.
+
+  - exploit unreachable_code_trueIsCalled; try eapply IC; eauto.
+    simpl in *; dcr; inv_get. assert (getAnn x0).
+    rewrite <- H4. eauto.
+    exploit compileF_get; eauto.
+    eapply Is_true_eq_true; eauto.
+    econstructor 2; [ | | ].
+    rewrite zip_app at 2; eauto with len.
+    rewrite take_app_lt; eauto 20 with len.
+    rewrite map_take. rewrite <- getAnn_eq; eauto.
+    rewrite <- map_take. eauto.
+    simpl.
+    eapply IH in H0; eauto.
+    eapply (IHCC _ _ _ (snd Zs)); eauto.
+Qed.
+
+Lemma DVE_callChain' RL ZL F als l' k
+      (IH : forall k Zs,
+          get F k Zs ->
+       forall (ZL : 〔params〕) (RL : 〔bool〕) (lv : ann bool) (n : nat),
+       unreachable_code SoundAndComplete ZL RL (snd Zs) lv ->
+       trueIsCalled (snd Zs) (LabI n) ->
+       getAnn lv ->
+       isCalled (compile (pair ⊜ RL ZL) (snd Zs) lv)
+                (LabI (countTrue (fst ⊝ take n (pair ⊜ RL ZL)))))
+  (LEN: ❬F❭ = ❬als❭)
+  (UCF:forall (n : nat) (Zs : params * stmt) (a : ann bool),
+       get F n Zs ->
+       get als n a ->
+       unreachable_code SoundAndComplete (fst ⊝ F ++ ZL)
+         (getAnn ⊝ als ++ RL) (snd Zs) a)
+  (Ann: get (getAnn ⊝ als ++ RL) l' true)
+  (CC: callChain trueIsCalled F (LabI l') (LabI k))
+: callChain isCalled
+            (compileF compile (pair ⊜ (getAnn ⊝ als ++ RL) (fst ⊝ F ++ ZL)) F als)
+            (LabI (countTrue (fst ⊝ take l' (pair ⊜ (getAnn ⊝ als ++ RL)
+                                                  (fst ⊝ F ++ ZL)))))
+            (LabI (countTrue (fst ⊝ take k (pair ⊜ (getAnn ⊝ als ++ RL)
+                                                  (fst ⊝ F ++ ZL))))).
+Proof.
+  general induction CC.
+  - econstructor.
+
+  - inv_get.
+    exploit unreachable_code_trueIsCalled; try eapply H0; eauto.
+    simpl in *; dcr; inv_get. assert (x0 = true).
+    destruct (getAnn x), x0; isabsurd; eauto.
+    exploit compileF_get; eauto.
+    econstructor 2; [ | | ].
+    rewrite zip_app at 2; eauto with len.
+    rewrite take_app_lt; eauto 20 with len.
+    rewrite map_take. rewrite <- getAnn_eq; eauto.
+    rewrite <- map_take. eauto.
+    simpl.
+    eapply IH in H0; eauto. rewrite <- H3. eauto.
+    subst. eauto.
+Qed.
+
 Lemma DVE_isCalled ZL RL s lv n
   : unreachable_code SoundAndComplete ZL RL s lv
     -> trueIsCalled s (LabI n)
     -> getAnn lv
-    -> isCalled (compile (pair ⊜ RL ZL) s lv) (LabI (countTrue (fst ⊝ take n (pair ⊜ RL ZL)))).
+    -> isCalled (compile (pair ⊜ RL ZL) s lv)
+               (LabI (countTrue (fst ⊝ take n (pair ⊜ RL ZL)))).
 Proof.
   intros Live IC.
   revert ZL RL lv n Live IC.
   sind s; simpl; intros; invt unreachable_code; invt trueIsCalled; simpl in *; eauto using isCalled.
   - repeat cases; eauto using isCalled.
   - repeat cases; eauto using isCalled.
-  - simpl in *.
-    general induction H7.
+  - eapply callChain_cases in H6. destruct H6; subst.
     + cases.
-      * exploit (IH s) as IHt; eauto.
+      * exploit (IH t) as IHt; eauto.
         rewrite <- zip_app; eauto with len.
         rewrite zip_app in IHt; eauto with len.
         rewrite take_app_ge in IHt; eauto 20 with len.
@@ -219,85 +330,69 @@ Proof.
         rewrite <- getAnn_eq in IHt; eauto.
         erewrite <- compileF_length in IHt; eauto.
         erewrite <- Heq in IHt. eauto.
-      * rewrite Heq. eapply IsCalledLet.
-        exploit (IH s) as IHt; eauto.
-        rewrite compileF_length; eauto.
+      * rewrite Heq. econstructor. econstructor 1.
+        exploit (IH t) as IHt; eauto.
+        rewrite <- zip_app; eauto with len.
+        rewrite compileF_length; eauto. simpl.
         rewrite zip_app in IHt; eauto with len.
         rewrite take_app_ge in IHt; eauto 20 with len.
         rewrite zip_length2 in IHt; eauto with len.
         rewrite map_length in IHt.
         orewrite (❬F❭ + n - ❬als❭ = n) in IHt. simpl.
         rewrite map_app in IHt. rewrite countTrue_app in IHt.
-        rewrite <- getAnn_eq in IHt; eauto.
-        econstructor; eauto.
-    + cases.
+        erewrite <- getAnn_eq in IHt; eauto.
+    + destruct H2 as [? [? [? ?]]]; dcr.
+      destruct l' as [l'].
+      cases.
       * exfalso. inv_get.
-        eapply trueIsCalled_compileF_not_nil; eauto.
-      * rewrite Heq; clear Heq. inv_get.
-        edestruct (unreachable_code_trueIsCalled H1 H); eauto; simpl in *; dcr.
-        inv_get. rewrite H10 in H5.
-        exploit compileF_get; eauto.
-        eapply Is_true_eq_true; eauto.
-        econstructor; eauto.
-      * rewrite compileF_length; eauto.
-        rewrite (take_eta k (getAnn ⊝ als)). rewrite countTrue_app.
-        rewrite map_take. erewrite <- get_eq_drop; eauto.
-        rewrite <- H5; simpl. omega.
-      * exploit IHIC1 as IH; eauto; try reflexivity; simpl.
-        rewrite compileF_length; eauto with len.
-        rewrite zip_app in IH; eauto with len.
-        rewrite take_app_ge in IH; eauto 20 with len.
-        rewrite map_app in IH.
-        rewrite <- getAnn_eq in IH; eauto. rewrite countTrue_app in IH; eauto.
-        rewrite zip_length2 in IH; eauto with len.
-        rewrite map_length in IH. orewrite (❬F❭ + n - ❬als❭ = n) in IH.
+        eapply get_in_range in H2. destruct H2. inv_get.
+        eapply trueIsCalled_compileF_not_nil.
+        eapply H0. eauto. eauto. eauto. eauto. eauto.
+      * rewrite Heq; clear Heq p b. inv_get.
         rewrite <- zip_app; eauto with len.
-      * exploit IHIC2 as IH; eauto.
-        rewrite zip_app in IH; eauto with len.
-        erewrite <- getAnn_take_eq in IH; eauto.
-  - cases.
-    + rewrite <- zip_app; eauto with len. exploit IHIC; eauto. reflexivity.
-      rewrite zip_app in H; eauto with len.
-      rewrite take_app_ge in H; eauto 20 with len.
-      rewrite zip_length2 in H; eauto with len.
-      rewrite map_length in H.
-      orewrite (❬F❭ + n - ❬als❭ = n) in H. simpl.
-      rewrite map_app in H. rewrite countTrue_app in H.
-      rewrite <- getAnn_eq in H; eauto.
-      erewrite <- compileF_length in H; eauto.
-      erewrite <- Heq in H. eauto.
-    + rewrite Heq. eapply IsCalledLet.
-      exploit IHIC; eauto; try reflexivity.
-      rewrite compileF_length; eauto.
-      rewrite zip_app in H; eauto with len.
-      rewrite take_app_ge in H; eauto 20 with len.
-      rewrite zip_length2 in H; eauto with len.
-      rewrite map_length in H.
-      orewrite (❬F❭ + n - ❬als❭ = n) in H. simpl.
-      rewrite map_app in H. rewrite countTrue_app in H.
-      rewrite <- getAnn_eq in H; eauto.
+        econstructor; eauto. simpl.
+        rewrite compileF_length; eauto.
+        eapply DVE_callChain; eauto.
 Qed.
 
 Lemma DVE_noUnreachableCode ZL RL s lv
-  : unreachable_code ZL RL s lv
+  : unreachable_code SoundAndComplete ZL RL s lv
+    -> getAnn lv
     -> noUnreachableCode (compile (pair ⊜ RL ZL) s lv).
 Proof.
-  intros Live. induction Live; simpl; repeat cases; eauto using noUnreachableCode.
+  intros Live GetAnn.
+  induction Live; simpl; repeat cases; eauto using noUnreachableCode.
+  - exploit H; try congruence; subst. eauto.
+  - specialize (H NOTCOND0). specialize (H0 NOTCOND). subst.
+    simpl in *. econstructor; eauto.
   - rewrite <- zip_app; eauto with len.
   - rewrite Heq; clear Heq.
     econstructor; eauto using noUnreachableCode.
     + intros. destruct Zs as [Z' s'].
       edestruct compileF_get_inv as [Zs' [a [n' ?]]]; eauto; dcr; subst; simpl.
+      simpl in *.
       rewrite <- zip_app; eauto with len.
+      eapply H2; eauto. rewrite H7; eauto.
     + rewrite <- zip_app; eauto with len.
-    + intros.
+    + intros. simpl in *.
       edestruct get_in_range as [Zs ?]; eauto. destruct Zs as [Z' s'].
-      edestruct compileF_get_inv as [Zs' [a [n' [lv' ?]]]]; eauto; dcr; subst; simpl.
-      exploit H2; eauto.
-      rewrite H7; eauto.
-      exploit DVE_isCalled as IH; eauto.
-      rewrite zip_app in IH; eauto with len.
-      erewrite <- getAnn_take_eq in IH; eauto.
+      edestruct compileF_get_inv as [Zs' [a [n' [lv' ?]]]]; eauto.
+      dcr; subst; simpl.
+      exploit H3 as ICF; eauto. rewrite H8; eauto.
+      rewrite <- zip_app; eauto with len.
+      destruct ICF as [[l'] [? ?]].
+      exploit DVE_isCalled; eauto.
+      eexists; split; eauto.
+      exploit DVE_callChain'; eauto using DVE_isCalled.
+      exploit unreachable_code_trueIsCalled; eauto.
+      dcr; subst; simpl in *. rewrite H12 in GetAnn.
+      destruct x; isabsurd; eauto.
+      rewrite zip_app in H9 at 3; [| eauto with len].
+      rewrite take_app_lt in H9.
+      setoid_rewrite map_take in H9 at 2.
+      rewrite <- getAnn_eq in H9; eauto.
+      setoid_rewrite <- map_take in H9. eauto.
+      eauto with len.
 Qed.
 
 Module I.
@@ -359,8 +454,8 @@ Proof.
 Qed.
 
 
-Lemma sim_I ZL RL r L L' V s a
-: unreachable_code ZL RL s a
+Lemma sim_I i ZL RL r L L' V s (a:ann bool) (Ann:getAnn a)
+  : unreachable_code i ZL RL s a
 -> simILabenv Bisim r SR (pair ⊜ RL ZL) L L'
 -> (forall (f:nat) Z,
       get (pair ⊜ RL ZL) f (true, Z)
@@ -377,7 +472,7 @@ Proof.
   - repeat cases.
     + edestruct (exp2bool_val2bool V); eauto; dcr.
       eapply sim'_expansion_closed.
-      eapply (IH s1); eauto.
+      eapply (IH s1); eauto. rewrite H5; eauto.
       eapply star2_silent.
       econstructor; eauto. eapply star2_refl.
       eapply star2_refl.
@@ -399,7 +494,8 @@ Proof.
       left; eapply (IH s2); eauto using agree_on_incl.
       pfold. econstructor 4; try eapply star2_refl; eauto.
       stuck. stuck.
-  - edestruct H1 as [? [? [GetL GetL']]]; eauto using zip_get.
+  - assert (b=true). destruct a0, b; isabsurd; eauto. subst.
+    edestruct H1 as [? [? [GetL GetL']]]; eauto using zip_get.
     remember (omap (exp_eval V) Y). symmetry in Heqo.
     destruct o.
     + destruct x as [Z1 s1 n1], x0 as [Z2 s2 n2].
@@ -426,15 +522,15 @@ Proof.
         eapply simILabenv_extension with (F':=nil); eauto. eauto with len.
         intros; isabsurd. isabsurd.
         simpl; intros; dcr; subst. exfalso.
-        rewrite get_app_lt in H9; eauto with len. inv_get.
-        assert (length (compileF compile (pair ⊜ (getAnn ⊝ als) (fst ⊝ s) ++ pair ⊜ RL ZL) s als)
+        rewrite get_app_lt in H8; eauto with len. inv_get.
+        assert (length (compileF compile (pair ⊜ (getAnn ⊝ als) (fst ⊝ F) ++ pair ⊜ RL ZL) F als)
                 <> 0). {
           rewrite compileF_length; eauto.
           eapply countTrue_exists. rewrite <- EQ1; eauto using map_get_1.
         }
         eapply H6. rewrite <- Heq. eauto.
         simpl; intros; dcr; subst.
-        rewrite get_app_ge in H9; eauto with len. inv_get.
+        rewrite get_app_ge in H8; eauto with len. inv_get.
         rewrite map_take. rewrite map_app.
         rewrite map_zip.
         rewrite zip_map_fst; eauto with len.
@@ -447,7 +543,7 @@ Proof.
       * intros. rewrite zip_app in H2; eauto with len.
         eapply get_app_cases in H2. destruct H2.
         exfalso. inv_get.
-        assert (length (compileF compile (pair ⊜ (getAnn ⊝ als) (fst ⊝ s) ++ pair ⊜ RL ZL) s als)
+        assert (length (compileF compile (pair ⊜ (getAnn ⊝ als) (fst ⊝ F) ++ pair ⊜ RL ZL) F als)
                 <> 0). {
           rewrite compileF_length; eauto.
           eapply countTrue_exists. rewrite <- EQ1; eauto using map_get_1.
@@ -469,14 +565,15 @@ Proof.
         + rewrite zip_app; eauto with len.
           eapply simILabenv_extension; eauto. eauto with len.
           * intros. hnf; intros.
-            hnf in H3. dcr. hnf in H11; dcr; subst.
+            hnf in H3. dcr. hnf in H10; dcr; subst.
             rewrite get_app_lt in H14; eauto using get_range.
             inv_get.
-            exploit (compileF_get ((pair ⊜ (getAnn ⊝ als) (fst ⊝ s) ++ pair ⊜ RL ZL) )); eauto.
+            exploit (compileF_get ((pair ⊜ (getAnn ⊝ als) (fst ⊝ F) ++ pair ⊜ RL ZL) )); eauto.
             erewrite <- getAnn_take_eq in H7; eauto.
             simpl in *. get_functional.
             rewrite <- zip_app; eauto with len.
-            eapply IH; eauto. exploit H8; eauto.
+            eapply IH; eauto. rewrite EQ; eauto.
+            exploit H9; eauto.
             rewrite zip_app; eauto with len.
             intros.
             eapply inv_extend; eauto with len.
@@ -484,12 +581,12 @@ Proof.
             hnf in H2. dcr; subst.
             rewrite get_app_lt in H12; eauto with len.
             inv_get. simpl; unfold ParamRel; simpl.
-            exploit (compileF_get ((pair ⊜ (getAnn ⊝ als) (fst ⊝ s) ++ pair ⊜ RL ZL) )); eauto.
+            exploit (compileF_get ((pair ⊜ (getAnn ⊝ als) (fst ⊝ F) ++ pair ⊜ RL ZL) )); eauto.
             erewrite <- getAnn_take_eq in H6; eauto.
             get_functional. eauto.
           * intros. rewrite compileF_length; eauto.
             hnf in H2; dcr; subst.
-            rewrite get_app_lt in H9;
+            rewrite get_app_lt in H8;
               [| rewrite zip_length2; eauto with len; rewrite map_length; omega].
             inv_get.
             erewrite <- getAnn_take_eq; eauto.
@@ -512,34 +609,14 @@ Proof.
       rewrite zip_app; eauto with len. intros; eapply inv_extend; eauto.
 Qed.
 
-Lemma sim_DVE V s a
-: unreachable_code nil nil s  a
--> @sim I.state _ I.state _ Bisim (nil,V, s) (nil,V, compile nil s a).
+Lemma sim_DVE i V s a
+  : unreachable_code i nil nil s a
+    -> getAnn a
+    -> @sim I.state _ I.state _ Bisim (nil,V, s) (nil,V, compile nil s a).
 Proof.
   intros. eapply sim'_sim.
-  eapply (@sim_I nil nil); eauto; isabsurd.
+  eapply (@sim_I i nil nil); eauto; isabsurd.
   econstructor; simpl; eauto using @sawtooth; isabsurd.
 Qed.
 
 End I.
-
-Fixpoint compile_live (s:stmt) (a:ann (set var)) : ann (set var) :=
-  match s, a with
-    | stmtLet x e s, ann1 lv an as a =>
-      ann1 lv (compile_live s an)
-    | stmtIf e s t, ann2 lv ans ant =>
-      if [exp2bool e = Some true] then
-        compile_live s ans
-      else if [exp2bool e = Some false ] then
-        compile_live t ant
-      else
-        ann2 lv (compile_live s ans) (compile_live t ant)
-    | stmtApp f Y, ann0 lv => ann0 lv
-    | stmtReturn x, ann0 lv => ann0 lv
-    | stmtExtern x f Y s, ann1 lv an as a =>
-      ann1 lv (compile_live s an)
-    | stmtFun F t, annF lv ans ant =>
-      let ans' := zip (fun Zs a => compile_live (snd Zs) a) F ans in
-      annF lv ans' (compile_live t ant)
-    | _, a => a
-  end.
